mppa_k1c/Asmblockgenproof.v
@@ -521,7 +521,7 @@ Proof.
     unfold transl_cond_float32. exploreInst; try discriminate.
     unfold transl_cond_notfloat32. exploreInst; try discriminate.
   - simpl in TIB. unfold transl_load in TIB. exploreInst; try discriminate.
-    all: monadInv TIB; unfold transl_memory_access in EQ0; unfold transl_memory_access2 in EQ0; exploreInst; try discriminate.
+    all: monadInv TIB; unfold transl_memory_access in EQ0; unfold transl_memory_access2 in EQ0; unfold transl_memory_access2XS in EQ0; exploreInst; try discriminate.
   - simpl in TIB. unfold transl_store in TIB. exploreInst; try discriminate.
     all: monadInv TIB; unfold transl_memory_access in EQ0; unfold transl_memory_access2 in EQ0; exploreInst; try discriminate.
 Qed.
